\def\duedate{10/14/22}
\def\HWnum{6}
\input{../preamble.tex}

\begin{document}
    
\prob{1}{
Which operators are linear?
}

a) $\displaystyle Au = -\partial^2u$, $\mathcal{D} = \{ u \in C^2[0,\pi] ~\big|~ u(0) = 0 ~{\rm and}~ u'(\pi)=0 \}$

This is a linear operator on the vector space $\mathcal{D}$ since
\begin{eqnarray}
    \label{eq:lin-op-a}
    A(\alpha u + \beta v) = -\partial^2 (\alpha u + \beta v) = \alpha(-\partial^2 u) + \beta (-\partial^2 v) = \alpha Au + \beta Av
.\end{eqnarray}

b) $\displaystyle Au = -\partial^2u$, $\mathcal{D} = \{ u \in C^2[0,\pi] ~\big|~ u(0) = 0 ~{\rm and}~ u'(\pi)=\pi \}$

The space $\mathcal{D}$ is not a proper vector space since if $u,v \in \mathcal{D}$, then $u + v \not\in \mathcal{D}$ since $u'(\pi) + v'(\pi) = 2\pi$.
Hence, $A$ is not a linear operator on the space $\mathcal{D}$ since $Au$ must be in the vector space $\mathcal{D}$ for all $u \in \mathcal{D}$.

c) $\displaystyle Au = u_{xx} + x^2u$, $\mathcal{D} = C^2(\reals)$ 

This is clearly a linear operator since
\begin{eqnarray}
    \label{eq:lin-op-c}
    A(\alpha u + \beta v) = \partial_{x}^2(\alpha u + \beta v) + x^2(\alpha u + \beta v) = \alpha[u_{xx} + x^2u] + \beta[v_{xx} + x^2v] = \alpha Au + \beta Av
.\end{eqnarray}

d) $Au = u_{xx} + u^2$, $\mathcal{D} = C^2(\reals)$ 

This is not a linear operator:
\begin{eqnarray}
    \label{eq:lin-op-d}
    A(\alpha u) = \alpha u_{xx} + \alpha^2 u^2 \ne \alpha Au
.\end{eqnarray}


\prob{2}{
Solve $u_{t} = 3u_{x} + 5u$, $u(x,0) = f(x)$.
}

We wish to solve the equation $u_{t} = Au$, where $A = 3\partial_{x} + 5$ and $u(x,0) = f(x)$, which has solution 
\begin{eqnarray}
    \label{eq:solve-t-eq}
    u = e^{tA} f(x) = e^{3t\partial_{x}}e^{5t} f(x) = e^{5t}f(x+3t)
.\end{eqnarray}


\prob{3}{
    Solve $u_{tt} - u_{xx} = 0$, $x \in \reals$, $t > 0$ for $u(x,0) = 3\sin{5x} - \cos{3x}$, $u_{t}(x,0) = 2x + 3x^2$. Find only $u(0,t)$.
}

The general solution to the wave equation $u_{tt} - c^2u_{xx} = 0$ with initial conditions $u(x,0) = \phi(x)$, $u_{t}(x,0) = \psi(x)$ is
\begin{eqnarray}
    \label{eq:gen-sol-wave}
    u(x,t) = \frac{1}{2}\big[ \phi(x + ct) + \phi(x - ct) \big] + \frac{1}{2c} \int_{x-ct}^{x+ct} \psi(s) \dd{s}
.\end{eqnarray}
Hence, for our problem, we have the solution
\begin{align}
    \label{eq:sol-3}
    u(x,t) &= \frac{1}{2}\big[ 3\sin{[5(x+t)]} - \cos{[3(x+t)]} + 3\sin{[5(x-t)]} - \cos{[3(x-t)]} \big] \notag \\
           &+ \frac{1}{2}\int_{x-t}^{x+t} (2s + 3s^2) \dd{s} \notag \\
           &= 3\cos{(5t)}\sin{(5x)} - \cos{(3t)}\cos{(3x)} \notag \\
           &+ \frac{1}{2}[(x+t)^2 - (x-t)^2 + (x+t)^3 - (x-t)^3] \notag \\
           &= \eqbox{3\cos{(5t)}\sin{(5x)} - \cos{(3t)}\cos{(3x)} + 2t(t^2 + 3x^2 + 2x)}
.\end{align}


\prob{4}{
Find $u(x,t)$ for the equation $u_{t} - ku_{xx} = 0$, $x \in \reals$, $t > 0$ subject to $u(x,0) = e^{-(x+1)^2}$.
}

We can find $u(x,t)$ subject to the initial condition as follows:
\begin{align}
    \label{eq:solve-u-diff}
    u(x,t) &= \frac{1}{\sqrt{4 \pi k t}} \int_{-\infty}^{\infty} e^{-(x-y)^2/4kt}e^{-(y+1)^2} \dd{y} \notag \\
           &= \frac{1}{\sqrt{4 \pi k t}} e^{-x^2/4kt - 1} \int_{-\infty}^{\infty} e^{-y^2/4kt - y^2 - 2y + xy/2kt} \dd{y} \notag \\
           &= \frac{1}{\sqrt{4 \pi k t}} e^{-x^2/4kt - 1} \int_{-\infty}^{\infty} e^{-(1 + 1/4kt)y^2 + 2(x/4kt - 1)y} \dd{y}
.\end{align}
Denote $a = 1 + 1/4kt$ and $b = x/4kt - 1$, then
\begin{align}
    \label{eq:u-diff-simplify}
    \int_{-\infty}^{\infty} e^{-(1 + 1/4kt)y^2 + 2(x/4kt - 1)y} \dd{y} &= \int_{-\infty}^{\infty} e^{-a(y^2 + 2by/a)} \dd{y} \notag \\
                                                                       &= e^{b^2/a} \int_{-\infty}^{\infty} e^{-a(y + b/a)^2} \dd{y} \notag \\
                                                                       &= e^{4kt(x/4kt - 1)^2/(1 + 4kt)} \sqrt{\frac{4 \pi k t}{1 + 4kt}}
.\end{align}
Finally, we have our solution:
\begin{eqnarray}
    \label{eq:solution-5}
    u(x,t) = \frac{1}{\sqrt{1 + 4kt}} e^{-(x+1)^2/(1 + 4kt)}
.\end{eqnarray}




\prob{5}{
    Find the Fourier transform $\displaystyle \widehat{f}(\omega) = \int_{-\infty}^{\infty} f(x)e^{-i\omega x} \dd{\omega}$ for $f(x) = xe^{-x^2}$.
}

The fourier transform of $f$ is given as
\begin{eqnarray}
    \label{eq:fourier-trans-f}
    \widehat{f}(\omega) = \int_{-\infty}^{\infty} xe^{-i\omega x} e^{-x^2} \dd{x} = \frac{i}{\omega} \dv{\omega} \int_{-\infty}^{\infty} e^{-i\omega x} e^{-x^2} \dd{\omega} = \frac{i}{\omega}\dv{\mathcal{F}\{\exp(-x^2)\}}{k}
.\end{eqnarray}
The fourier transform of this ``gaussian'' is as follows
\begin{align}
    \label{eq:fourier-trans-gauss}
    \mathcal{F}\{ e^{-x^2} \} &= \int_{-\infty}^{\infty} e^{-i\omega x} e^{-x^2} \dd{x} = \int_{-\infty}^{\infty} e^{-(x^2 + i\omega)} \dd{x} \notag \\
                              &= e^{-\omega^2/4} \int_{-\infty}^{\infty} e^{-(x + i\omega/2)^2} \dd{x} = \sqrt{\pi} e^{-\omega^2/4}
.\end{align}
Thus,
\begin{eqnarray}
    \label{eq:fourier-deriv}
    \widehat{f}(\omega) = \frac{i\sqrt{\pi}}{\omega} \Big( -\frac{\omega}{2} e^{-\omega^2/4} \Big) = -\frac{i\sqrt{\pi}}{2} e^{-\omega^2/4}
.\end{eqnarray}


\prob{6*}{
    Find the Fourier transform for $f(x) = -H(x+1) + 2H(x) - H(x-1)$, where \\ $\displaystyle H(x) = \begin{cases} 1, & x \geq 0 \\ 0, & x < 0\end{cases}$.
}



\prob{7*}{
Solve $u_{t} = 5u_{x} - 3xu + u$, $x \in \reals$, $t > 0$ with $u(x,0) = f(x)$.
Display the graph of $f(x)$.
}



\end{document}
